Fix to compile

src/semantics/Linking.v
@@ -106,89 +106,6 @@ Module OMod.
 End OMod.
 
 
-Definition StateL
-           (S V: Type) (l: Lens.t S V)
-           (X: Type)
-           (run: V -> V * X): sE S X :=
-  State (lens_state l run).
-Arguments StateL: simpl never.
-
-Lemma StateL_id S X (run: S -> S * X):
-  State run = StateL Lens.id run.
-Proof.
-  unfold StateL, lens_state. f_equal. extensionality s.
-  unfold Lens.set,  Lens.view. ss.
-  apply surjective_pairing.
-Qed.
-
-Lemma StateL_compose S V W
-      (l0: Lens.t S V)
-      (l1: Lens.t V W)
-      X (run: W -> W * X):
-  map_lens l
-
-    StateL (Lens.compose l0 l1) run = map_lens l State run.
-Proof.
-  unfold StateL, lens_state. f_equal. extensionality s.
-  unfold Lens.set,  Lens.view. ss.
-  symmetry. apply surjective_pairing.
-Qed.
-
-Coq
-
-Definition GetL
-           (S V: Type) (l: Lens.t S V)
-           (X: Type)
-           (pr: V -> X): sE S X :=
-  Get (pr ∘ Lens.view l).
-Arguments GetL: simpl never.
-
-Definition ModifyL
-           (S V: Type) (l: Lens.t S V)
-           (X: Type)
-           (f: V -> V): sE S unit :=
-  Modify (Lens.modify l f).
-Arguments ModifyL: simpl never.
-
-Lemma
-
-
-  Lemma map_event_plmap_modify_nocont
-    (f : state -> state)
-    : map_event (plmap p l) (trigger (Modify f)) = trigger (Modify (Lens.modify l f)).
-  Proof.
-    unfold trigger. rewrite map_event_vis. rewrite <- map_lens_Modify.
-    eapply observe_eta; ss. f_equal. extensionalities x.
-    eapply map_event_ret.
-  Qed.
-
-
-
-  Lemma map_event_plmap_get_nocont
-    X (pr : state -> X)
-    : map_event (plmap p l) (trigger (Get pr)) = trigger (Get (pr ∘ Lens.view l)).
-  Proof.
-    unfold trigger. rewrite map_event_vis. rewrite <- map_lens_Get.
-    eapply observe_eta; ss. f_equal. extensionalities x.
-    eapply map_event_ret.
-  Qed.
-
-
-plmap
-
-  (* sE is just state monad *)
-  Variant sE (S : Type) (X : Type) : Type :=
-  | State (run : S -> S * X) : sE S X
-  .
-
-  Variant callE: Type -> Type :=
-  | Call (fn: fname) (arg: Any.t): callE Any.t
-  .
-
-  Definition Get {S} {X} (p : S -> X) : sE S X := State (fun x => (x, p x)).
-  Definition Modify {S} (f : S -> S) : sE S () := State (fun x => (f x, tt)).
-
-
 Section RED.
 
   Import OMod.
@@ -318,6 +235,17 @@ Section RED.
     @close_itree omd md R (trigger (Get p) >>= ktr) =
       x <- trigger (Get (p ∘ Lens.view fstl));; tau;; close_itree omd md (ktr x).
   Proof. rewrite ! bind_trigger. eapply close_itree_vis_get. Qed.
+
+  Lemma close_itree_trigger_sE
+        omd md
+        R
+        X (se: @sE omd.(Mod.state) X) ktr
+    :
+    @close_itree omd md R (trigger se >>= ktr) =
+      x <- trigger (map_lens fstl se);; tau;; close_itree omd md (ktr x).
+  Proof.
+    destruct se. rewrite close_itree_trigger_state. ss.
+  Qed.
 
   Lemma close_itree_vis_call
         omd md
